make implict fields also optional

Proto3.fst
@@ -14,19 +14,22 @@ module List = FStar.List.Tot
 
 type byte = String.char
 type bytes = list byte
+let empty_bytes : bytes = []
 
 type width = z:int{z = 32 \/ z = 64}
 type zw (w:width) = z:int{- pow2 (w-1) <= z /\ z < pow2 (w-1) } 
+let zwz (w:width) : zw w = 0
 type uw (w:width) = n:nat{n < pow2 w}
+let uwz (w:width) : uw w = 0
  
 type proto_dec (a:Type) = 
-| IMPLICIT : a -> proto_dec a
+| IMPLICIT : option a -> proto_dec a
 | OPTIONAL : option a -> proto_dec a
 | REPEATED : list a -> proto_dec a
 
 let is_IMPLICIT_v (#t:eqtype) (d:proto_dec t) (v:t) : bool = 
   match d with 
-  | IMPLICIT e -> e = v
+  | IMPLICIT (Some e) -> e = v
   | _ -> false
 
 let is_OPTIONAL_v (#t:eqtype) (d:proto_dec t) (v:t) : bool = 
@@ -41,7 +44,7 @@ let is_REPEATED_v (#t:eqtype) (d:proto_dec t) (v:list t) : bool =
 
 type proto_ty = 
 | DOUBLE // I would add a double here, but F* literally doesn't support any kind of floating point number...
-| FLOAT // See above.
+| FLOAT  // See above.
 | INT :    w:width -> proto_dec (zw w) -> proto_ty
 | UINT :   w:width -> proto_dec (uw w) -> proto_ty
 | SINT :   w:width -> proto_dec (zw w) -> proto_ty
@@ -102,15 +105,17 @@ let sint_int (w:width) (v:zw w) : zw w = if -(pow2 (w-2)) <= v && v < pow2 (w-2)
   else 
       2 * (abs v) - pow2 w - idn (v < 0)
 
-let pty_wrap (#t1:Type) (#t2:Type) (f:t1 -> t2) (a:proto_dec t1) = 
+let pty_wrap (#t1:Type) (#t2:Type) (f:t1 -> t2) (d:t2) (a:proto_dec t1) = 
   match a with 
-  | IMPLICIT a' -> IMPLICIT (f a')
+  | IMPLICIT (Some a') -> IMPLICIT (Some (f a'))
+  | IMPLICIT None -> IMPLICIT (Some d)
   | OPTIONAL (Some a') -> OPTIONAL (Some (f a'))
   | OPTIONAL None -> OPTIONAL None 
   | REPEATED l -> REPEATED (List.map f l)
 
-let proto_ty_int_sint32 = pty_wrap (int_sint 32)
-let proto_ty_int_sint_test_i = proto_ty_int_sint32 (IMPLICIT (-9))
+let proto_ty_int_sint32 = pty_wrap (int_sint 32) (zwz 32)
+let proto_ty_int_sint_test_i = proto_ty_int_sint32 (IMPLICIT (Some (-9)))
+let proto_ty_int_sint_test_i' = proto_ty_int_sint32 (IMPLICIT (None))
 let proto_ty_int_sint_test_o = proto_ty_int_sint32 (OPTIONAL None)
 let proto_ty_int_sint_test_o' = proto_ty_int_sint32 (OPTIONAL (Some 9))
 let proto_ty_int_sint_test_r = proto_ty_int_sint32 (REPEATED [(-9); 9])
@@ -130,84 +135,84 @@ type val_rel : proto_ty -> proto_ty -> Type =
   // Rules from the original value relation
   | ValStrByt : 
     v1:(proto_dec string) -> 
-    v2:(proto_dec bytes){v2 = pty_wrap String.list_of_string v1} -> 
+    v2:(proto_dec bytes){v2 = pty_wrap String.list_of_string empty_bytes v1} -> 
     val_rel (STRING v1) (BYTES v2)
   | ValBytStr : 
     v1:(proto_dec bytes) ->
-    v2:(proto_dec string){v2 = pty_wrap String.string_of_list v1} ->
+    v2:(proto_dec string){v2 = pty_wrap String.string_of_list "" v1} ->
     val_rel (BYTES v1) (STRING v2)
   | ValUintChgW : 
     #w1:width ->
     #w2:width ->
     v1:(proto_dec (uw w1)) ->
-    v2:(proto_dec (uw w2)){v2 = pty_wrap (uint_change_w w2) v1} ->
+    v2:(proto_dec (uw w2)){v2 = pty_wrap (uint_change_w w2) (uwz w2) v1} ->
     val_rel (UINT w1 v1) (UINT w2 v2)
   | ValIntChgW : 
     #w1:width ->
     #w2:width ->
     v1:(proto_dec (zw w1)) ->
-    v2:(proto_dec (zw w2)){v2 = pty_wrap (int_change_w w2) v1} ->
+    v2:(proto_dec (zw w2)){v2 = pty_wrap (int_change_w w2) (zwz w2) v1} ->
     val_rel (INT w1 v1) (INT w2 v2)
   | ValSintChgW :
     #w1:width ->
     #w2:width ->
     v1:(proto_dec (zw w1)) ->
-    v2:(proto_dec (zw w2)){v2 = pty_wrap (int_change_w w2) v1} ->
+    v2:(proto_dec (zw w2)){v2 = pty_wrap (int_change_w w2) (zwz w2) v1} ->
     val_rel (SINT w1 v1) (SINT w2 v2)
   | ValUintInt : 
     #w:width ->
     v1:(proto_dec (uw w)) ->
-    v2:(proto_dec (zw w)){v2 = pty_wrap (uint_int w) v1} -> 
+    v2:(proto_dec (zw w)){v2 = pty_wrap (uint_int w) (zwz w) v1} -> 
     val_rel (UINT w v1) (INT w v2)
   | ValIntUint : 
     #w:width ->
     v1:(proto_dec (zw w)) ->
-    v2:(proto_dec (uw w)){v2 = pty_wrap (int_uint w) v1} -> 
+    v2:(proto_dec (uw w)){v2 = pty_wrap (int_uint w) (uwz w) v1} -> 
     val_rel (INT w v1) (UINT w v2)
   | ValUintSint : 
     #w:width ->
     v1:(proto_dec (uw w)) ->
-    v2:(proto_dec (zw w)){v2 = pty_wrap (uint_sint w) v1} -> 
+    v2:(proto_dec (zw w)){v2 = pty_wrap (uint_sint w) (zwz w) v1} -> 
     val_rel (UINT w v1) (INT w v2)
   | ValIntSint : 
     #w:width ->
     v1:(proto_dec (zw w)) ->
-    v2:(proto_dec (zw w)){v2 = pty_wrap (int_sint w) v1} -> 
+    v2:(proto_dec (zw w)){v2 = pty_wrap (int_sint w) (zwz w) v1} -> 
     val_rel (INT w v1) (SINT w v2)
   | ValSintInt : 
     #w:width ->
     v1:(proto_dec (zw w)) ->
-    v2:(proto_dec (zw w)){v2 = pty_wrap (int_sint w) v1} -> 
+    v2:(proto_dec (zw w)){v2 = pty_wrap (int_sint w) (zwz w) v1} -> 
     val_rel (SINT w v1) (INT w v2)
   | ValUintBool :
     #w:width ->
     v1:(proto_dec (uw w)) ->
-    v2:(proto_dec bool){v2 = pty_wrap (fun (u:uw w) -> u <> 0) v1} ->
+    v2:(proto_dec bool){v2 = pty_wrap (fun (u:uw w) -> u <> 0) false v1} ->
     val_rel (UINT w v1) (BOOL v2)
   | ValBoolUint :
     #w:width ->
     v1:(proto_dec bool) ->
-    v2:(proto_dec (uw w)){v2 = pty_wrap (idnuw w) v1} ->
+    v2:(proto_dec (uw w)){v2 = pty_wrap (idnuw w) (uwz w) v1} ->
     val_rel (BOOL v1) (UINT w v2)
   | ValIntBool : 
     #w:width ->
     v1:(proto_dec (zw w)) ->
-    v2:(proto_dec bool){v2 = pty_wrap (fun (u:zw w) -> u <> 0) v1} ->
+    v2:(proto_dec bool){v2 = pty_wrap (fun (u:zw w) -> u <> 0) false v1} ->
     val_rel (INT w v1) (BOOL v2)
   | ValBoolInt :
     #w:width ->
     v1:(proto_dec bool) ->
-    v2:(proto_dec (zw w)){v2 = pty_wrap (idnzw w) v1} ->
+    v2:(proto_dec (zw w)){v2 = pty_wrap (idnzw w) (zwz w) v1} ->
     val_rel (BOOL v1) (INT w v2)
   | ValSintBool : 
     #w:width ->
     v1:(proto_dec (zw w)) ->
-    v2:(proto_dec bool){v2 = pty_wrap (fun (u:zw w) -> u <> 0) v1} ->
+    v2:(proto_dec bool){v2 = pty_wrap (fun (u:zw w) -> u <> 0) false v1} ->
     val_rel (SINT w v1) (BOOL v2)
   | ValBoolSint :
     #w:width ->
     v1:(proto_dec bool) ->
-    v2:(proto_dec (zw w)){v2 = pty_wrap (idnzw w) v1} ->
+    v2:(proto_dec (zw w)){v2 = pty_wrap (idnzw w) (zwz w) v1} ->
     val_rel (BOOL v1) (SINT w v2)
   // Rules for dealing with modifiers 
   | ValAddOpt :
@@ -215,13 +220,13 @@ type val_rel : proto_ty -> proto_ty -> Type =
     #pty:(proto_dec t -> proto_ty) ->
     #v:t ->
     pty1:(proto_dec t){is_IMPLICIT_v pty1 v} ->
-    val_rel (pty (IMPLICIT v)) (pty (OPTIONAL (Some v)))
+    val_rel (pty (IMPLICIT (Some v))) (pty (OPTIONAL (Some v)))
   | ValRmOpt :
     #t:eqtype ->
     #pty:(proto_dec t -> proto_ty) ->
     #v:t ->
     pty1:(proto_dec t){is_OPTIONAL_v pty1 v} ->
-    val_rel (pty (OPTIONAL (Some v))) (pty (IMPLICIT v))
+    val_rel (pty (OPTIONAL (Some v))) (pty (IMPLICIT (Some v)))
   | ValAddRep :
     #t:eqtype ->
     #pty:(proto_dec t -> proto_ty) ->
@@ -229,33 +234,32 @@ type val_rel : proto_ty -> proto_ty -> Type =
     pty1:(proto_dec t){is_IMPLICIT_v pty1 v \/ is_OPTIONAL_v pty1 v} ->
     val_rel (pty pty1) (pty (REPEATED [v]))
     
-
 let test_str = "test"
 let test_bytes = String.list_of_string test_str
 
-val test_str_byt : val_rel (STRING (IMPLICIT test_str)) (BYTES (IMPLICIT test_bytes))
-let test_str_byt = ValStrByt (IMPLICIT test_str) (IMPLICIT test_bytes)
+val test_str_byt : val_rel (STRING (IMPLICIT (Some test_str))) (BYTES (IMPLICIT (Some test_bytes)))
+let test_str_byt = ValStrByt (IMPLICIT (Some test_str)) (IMPLICIT (Some test_bytes))
 
 val test_uint_demotion : val_rel (UINT 64 (OPTIONAL (Some 34359738370))) (UINT 32 (OPTIONAL (Some 2)))
 let test_uint_demotion = ValUintChgW (OPTIONAL (Some 34359738370)) (OPTIONAL (Some 2))
 
-val test_uint_int : val_rel (UINT 32 (IMPLICIT 2147483656)) (INT 32 (IMPLICIT (-2147483640)))
-let test_uint_int = ValUintInt (IMPLICIT 2147483656) (IMPLICIT (-2147483640))
+val test_uint_int : val_rel (UINT 32 (IMPLICIT (Some 2147483656))) (INT 32 (IMPLICIT (Some (-2147483640))))
+let test_uint_int = ValUintInt (IMPLICIT (Some 2147483656)) (IMPLICIT (Some (-2147483640)))
 
-val test_uint_big_int : val_rel (UINT 32 (IMPLICIT 2147483656)) (INT 64 (IMPLICIT (-2147483640)))
-let test_uint_big_int = ValTrans test_uint_int (ValIntChgW (IMPLICIT (-2147483640)) (IMPLICIT (-2147483640)))
+val test_uint_big_int : val_rel (UINT 32 (IMPLICIT (Some 2147483656))) (INT 64 (IMPLICIT (Some (-2147483640))))
+let test_uint_big_int = ValTrans test_uint_int (ValIntChgW (IMPLICIT (Some (-2147483640))) (IMPLICIT (Some (-2147483640))))
 
-val test_refl : val_rel (UINT 32 (IMPLICIT 0)) (UINT 32 (IMPLICIT 0))
-let test_refl = ValRefl (UINT 32 (IMPLICIT 0))
+val test_refl : val_rel (UINT 32 (IMPLICIT (Some 0))) (UINT 32 (IMPLICIT (Some 0)))
+let test_refl = ValRefl (UINT 32 (IMPLICIT (Some 0)))
 
-val test_add_opt : val_rel (UINT 32 (IMPLICIT 0)) (UINT 32 (OPTIONAL (Some 0)))
-let test_add_opt = ValAddOpt (IMPLICIT 0)
+val test_add_opt : val_rel (UINT 32 (IMPLICIT (Some 0))) (UINT 32 (OPTIONAL (Some 0)))
+let test_add_opt = ValAddOpt (IMPLICIT (Some 0))
 
-val test_rm_opt : val_rel (SINT 64 (OPTIONAL (Some 123456))) (SINT 64 (IMPLICIT 123456))
+val test_rm_opt : val_rel (SINT 64 (OPTIONAL (Some 123456))) (SINT 64 (IMPLICIT (Some 123456)))
 let test_rm_opt = ValRmOpt (OPTIONAL (Some 123456))
 
-val test_add_rep : val_rel (UINT 32 (IMPLICIT 12)) (UINT 32 (REPEATED [12]))
-let test_add_rep = ValAddRep (IMPLICIT 12)
+val test_add_rep : val_rel (UINT 32 (IMPLICIT (Some 12))) (UINT 32 (REPEATED [12]))
+let test_add_rep = ValAddRep (IMPLICIT (Some 12))
 
 val test_add_rep' : val_rel (INT 32 (OPTIONAL (Some (-23)))) (INT 32 (REPEATED [-23]))
 let test_add_rep' = ValAddRep (OPTIONAL (Some (-23)))
